src/program_proof/twophase/twophase_refinement_proof.v
@@ -1,9 +1,9 @@
 From Perennial.goose_lang.lib Require Import encoding crash_lock.
 From Perennial.program_proof Require Import proof_prelude.
 From Perennial.program_proof Require Import disk_lib.
-From Perennial.program_proof Require Import twophase.typed_translate twophase.wrapper_proof twophase.twophase_refinement_defs.
+From Perennial.program_proof Require Import twophase.typed_translate twophase.wrapper_proof twophase.twophase_refinement_defs twophase.twophase_sub_logical_reln_defs.
 From Perennial.goose_lang.ffi Require Import jrnl_ffi.
-From Perennial.goose_lang Require Import logical_reln_defns logical_reln_adeq spec_assert.
+From Perennial.goose_lang Require Import logical_reln_defns logical_reln_adeq spec_assert metatheory.
 From Perennial.program_logic Require Import ghost_var.
 
 From Goose Require github_com.mit_pdos.goose_nfsd.txn.
@@ -12,6 +12,7 @@ Existing Instances jrnl_spec_ext jrnl_spec_ffi_model jrnl_spec_ext_semantics jrn
 
 Section refinement.
 Context {PARAMS : jrnlInit_params}.
+Context (N : namespace).
 
 Notation jrnl_nat_K :=
 (leibnizO (nat * ((@spec_lang jrnl_spec_ext jrnl_spec_ffi_model jrnl_spec_ext_semantics).(language.expr)
@@ -58,11 +59,121 @@ Proof.
   iIntros (? hG hRG hJrnl) "Hinv Hcrash_cond".
 Admitted.
 
+Lemma jrnl_inv_twophase_pre `{hBuf: sep_buftxn_invariant.buftxnG Σ} {hG: heapG Σ} {hRG: refinement_heapG Σ}
+      {hJrnl : twophase_refinement_defs.jrnlG Σ} vs v:
+    jrnl_inv -∗
+    val_interp (smodel := jrnlTy_model) (hS := hJrnl) (@extT jrnl_val_ty JrnlT) vs v -∗
+    ∃ (l : loc) γ γ' objs_dom dinit, ⌜ v = #l ⌝ ∗ is_twophase_pre N l γ γ' dinit objs_dom.
+  Admitted.
+
+Ltac unfold_expr_vars :=
+    match goal with
+    | [ H : _ ∉ expr_vars _ |- _ ] => rewrite /expr_vars -/expr_vars in H
+    | [ H : _ ∉ val_vars _ |- _ ] => rewrite /val_vars -/val_vars in H
+    end.
+
+Lemma atomic_body_expr_subst :
+  ∀ Γ x e e' t v,
+    x ∉ dom (gset string) Γ →
+    x ∉ expr_vars e →
+    atomic_body_expr_transTy Γ (Var x) e e' t →
+    atomic_body_expr_transTy Γ (of_val v) e (subst x v e') t.
+Proof.
+  intros ?????? Hnot_in1 Hnot_in2 Htyping.
+  remember (Var x) as tph' eqn:Heq. revert Hnot_in1 Hnot_in2. revert Heq.
+  induction Htyping using @expr_typing_ind with
+      (P := (λ Γ tph' es e t
+               (HTYPE: atomic_body_expr_transTy Γ tph' es e t),
+             tph' = Var x →
+             x ∉ dom (gset string) Γ →
+             x ∉ expr_vars es →
+             atomic_body_expr_transTy Γ (of_val v) es (subst x v e) t))
+      (P0 := (λ Γ tph' vs vi t
+              (HTYPE: atomic_body_val_transTy Γ tph' vs vi t),
+              tph' = Var x →
+              x ∉ dom (gset string) Γ →
+              x ∉ val_vars vs →
+              atomic_body_val_transTy Γ (of_val v) vs vi t));
+    try (intros; subst; simpl; econstructor; eauto; done);
+    try (intros; subst; simpl;
+         econstructor; eauto;
+         [ eapply IHHtyping1; eauto; unfold_expr_vars; set_solver |
+           eapply IHHtyping2; eauto; unfold_expr_vars; set_solver ]; done);
+    try (intros; subst; simpl;
+         econstructor; eauto;
+         [ eapply IHHtyping1; eauto; unfold_expr_vars; set_solver |
+           eapply IHHtyping2; eauto; unfold_expr_vars; set_solver |
+           eapply IHHtyping3; eauto; unfold_expr_vars; set_solver ]; done).
+  - intros. subst. simpl.
+    destruct (decide _).
+    * subst; try econstructor; eauto.
+      exfalso. eapply H1. set_solver.
+    * econstructor. eauto.
+  - intros; subst; simpl.
+    econstructor; eauto.
+    rewrite decide_True.
+    { eapply IHHtyping; eauto; rewrite /expr_vars -/expr_vars //= in H1; destruct f; destruct x0 => //=;
+      rewrite //= in H1; rewrite /insert/ctx_insert ?dom_insert; set_solver. }
+    { rewrite /expr_vars -/expr_vars //= in H1. destruct f, x0; set_solver. }
+  - intros; subst; simpl.
+    rewrite decide_True //.
+    econstructor.
+    * eapply IHHtyping1; eauto; unfold_expr_vars; set_solver.
+    * eapply IHHtyping2; eauto; unfold_expr_vars; set_solver.
+  - intros; subst; simpl.
+    rewrite decide_True //.
+    econstructor.
+    * eapply IHHtyping1; eauto; unfold_expr_vars; set_solver.
+    * eapply IHHtyping2; eauto; unfold_expr_vars; set_solver.
+  - intros; subst; simpl.
+    econstructor.
+    * eapply IHHtyping; eauto. unfold_expr_vars; set_solver.
+    * eapply IHHtyping0; eauto; unfold_expr_vars; set_solver.
+  - intros; subst; simpl.
+    econstructor.
+    * eapply IHHtyping; eauto. unfold_expr_vars; set_solver.
+    * eapply IHHtyping0; eauto; unfold_expr_vars; set_solver.
+Qed.
+
 Lemma jrnl_atomic_obligation:
   @sty_atomic_obligation _ _ disk_semantics _ _ _ _ _ _ jrnlTy_model jrnl_atomic_transTy.
 Proof.
   rewrite /sty_atomic_obligation//=.
   iIntros (? hG hRG hJrnl el1 el2 tl e1 e2 t Γsubst Htrans) "Hinv Hspec Htrace HΓ HhasTy".
+  iIntros (j K Hctx) "Hj".
+  inversion Htrans; subst.
+  simpl.
+  rewrite lookup_delete.
+  rewrite -fmap_delete.
+  rewrite ?delete_notin; last first.
+  { apply not_elem_of_dom. erewrite <-dom_fmap. eauto. }
+
+  wpc_bind (subst_map _ el2).
+  spec_bind (subst_map _ el1) as Hctx.
+  iDestruct ("HhasTy" with "[//] Hj") as "H".
+  rewrite /sty_lvl_ops/=.
+  iApply (wpc_strong_mono with "H"); auto.
+  iSplit; last by (iModIntro; eauto).
+  iIntros (v) "Hv". iModIntro.
+  wpc_bind (op_wrappers.TwoPhase__Begin' v).
+  iApply wp_wpc.
+  iDestruct "Hv" as (vs) "(Hj&Hinterp)".
+  iDestruct (jrnl_inv_twophase_pre with "[$] [$]") as "H".
+  iDestruct "H" as (l γ γ' ?? ->) "H".
+  wp_apply (wp_TwoPhase__Begin' with "[$]").
+  iIntros (tph_val) "Hstarted".
+  iApply wp_wpc.
+  wp_pures.
+  rewrite decide_True //.
+  wp_pures.
+  apply (atomic_body_expr_subst _ _ _ _ _ #tph_val) in H2; swap 1 3.
+  { eauto. }
+  { intros Hin. eapply H0. rewrite elem_of_dom in Hin *.
+    intros (v&?). apply: elem_of_dom_2. eapply H; eauto. }
+  wp_bind (subst _ _ _).
+  rewrite subst_map_subst_comm //; last first.
+  { rewrite dom_fmap. rewrite dom_fmap in H0 *. eauto. }
+  (* Apply the fundamental lemma here *)
 Admitted.
 
 Existing Instances jrnl_semantics.
